

> restart;  
with(Physics) :

$$\begin{aligned} > ds^2 := \frac{(r-2m) dt^2}{r} - \frac{r dr^2}{r-2m} - r^2 (d\theta^2 + \sin(\theta)^2 d\phi^2) \\ ds^2 &:= \frac{(r-2m) dt^2}{r} - \frac{r dr^2}{r-2m} - r^2 (d\theta^2 + \sin(\theta)^2 d\phi^2) \end{aligned} \quad (1)$$

$$\begin{aligned} > ds^2 := -e^{v(r)} dt^2 + \frac{dr^2}{1 - \frac{b(r)}{r}} + r^2 (d\theta^2 + \sin(\theta)^2 d\phi^2) \\ ds^2 &:= -e^{v(r)} dt^2 + \frac{dr^2}{1 - \frac{b(r)}{r}} + r^2 (d\theta^2 + \sin(\theta)^2 d\phi^2) \end{aligned} \quad (2)$$

> Setup(coordinates = spherical, signature = '+ + + -', metric = ds^2)  
Default differentiation variables for d\_, D\_ and dAlembertian are: {X = (r, θ, ϕ, t)}  
Systems of spacetime coordinates are: {X = (r, θ, ϕ, t)}

$$\left[ \begin{aligned} &coordinatesystems = \{X\}, metric = \left\{ (1,1) = \frac{1}{1 - \frac{b(r)}{r}}, (2,2) = r^2, (3,3) = r^2 \sin(\theta)^2, (4, \right. \\ &\left. 4) = -e^{v(r)} \right\}, signature = + + + - \end{aligned} \right] \quad (3)$$

$$\begin{aligned} > g_{[\ ]} \\ g_{\mu, \nu} &= \begin{bmatrix} \frac{r}{r-b(r)} & 0 & 0 & 0 \\ 0 & r^2 & 0 & 0 \\ 0 & 0 & r^2 \sin(\theta)^2 & 0 \\ 0 & 0 & 0 & -e^{v(r)} \end{bmatrix} \end{aligned} \quad (4)$$

$$\begin{aligned} > g_{[\sim]} \\ g^{\mu, \nu} &= \begin{bmatrix} \frac{r-b(r)}{r} & 0 & 0 & 0 \\ 0 & \frac{1}{r^2} & 0 & 0 \\ 0 & 0 & \frac{1}{r^2 \sin(\theta)^2} & 0 \\ 0 & 0 & 0 & -e^{-v(r)} \end{bmatrix} \end{aligned} \quad (5)$$

> g\_[mu, ~nu, matrix]

$$\delta_{\mu}^{\nu} = \begin{bmatrix} 1 & 0 & 0 & 0 \\ 0 & 1 & 0 & 0 \\ 0 & 0 & 1 & 0 \\ 0 & 0 & 0 & 1 \end{bmatrix} \quad (6)$$

>  $g\_ [lineelement]$

$$\frac{r \mathbf{d}(r)^2}{r - b(r)} + r^2 \mathbf{d}(\theta)^2 + r^2 \sin(\theta)^2 \mathbf{d}(\phi)^2 - e^{v(r)} \mathbf{d}(t)^2 \quad (7)$$

>  $Christoffel[\mu, \alpha, \beta] = convert(Christoffel[\mu, \alpha, \beta], g\_)$

$$\Gamma_{\mu, \alpha, \beta} = \frac{\partial_{\beta}(g_{\alpha, \mu})}{2} + \frac{\partial_{\alpha}(g_{\beta, \mu})}{2} - \frac{\partial_{\mu}(g_{\alpha, \beta})}{2} \quad (8)$$

>  $seq(Christoffel[\sim mu, alpha, beta, matrix], \sim mu = [\sim 1, \sim 2, \sim 3, \sim 0])$

$$\Gamma_{\alpha, \beta}^1 = \left[ \left[ \frac{\left( \frac{d}{dr} b(r) \right) r - b(r)}{2 r (r - b(r))}, 0, 0, 0 \right], \right. \quad (9)$$

$$\left[ 0, -r + b(r), 0, 0 \right],$$

$$\left[ 0, 0, (-r + b(r)) \sin(\theta)^2, 0 \right],$$

$$\left[ 0, 0, 0, -\frac{(-r + b(r)) \left( \frac{d}{dr} v(r) \right) e^{v(r)}}{2 r} \right] \right], \Gamma_{\alpha, \beta}^2$$

$$= \begin{bmatrix} 0 & \frac{1}{r} & 0 & 0 \\ \frac{1}{r} & 0 & 0 & 0 \\ 0 & 0 & -\sin(\theta) \cos(\theta) & 0 \\ 0 & 0 & 0 & 0 \end{bmatrix}, \Gamma_{\alpha, \beta}^3 = \begin{bmatrix} 0 & 0 & \frac{1}{r} & 0 \\ 0 & 0 & \frac{\cos(\theta)}{\sin(\theta)} & 0 \\ \frac{1}{r} & \frac{\cos(\theta)}{\sin(\theta)} & 0 & 0 \\ 0 & 0 & 0 & 0 \end{bmatrix}, \Gamma_{\alpha, \beta}^4$$

$$= \begin{bmatrix} 0 & 0 & 0 & \frac{\frac{d}{dr} v(r)}{2} \\ 0 & 0 & 0 & 0 \\ 0 & 0 & 0 & 0 \\ \frac{\frac{d}{dr} v(r)}{2} & 0 & 0 & 0 \end{bmatrix}$$

> *Christoffel[nonzero]*

$$\begin{aligned} \Gamma_{\alpha, \mu, \nu} &= \left\{ (1, 1, 1) = \frac{\left(\frac{d}{dr} b(r)\right) r - b(r)}{2 (r - b(r))^2}, (1, 2, 2) = -r, (1, 3, 3) = -r \sin(\theta)^2, (1, 4, 4) \right. \\ &= \frac{\left(\frac{d}{dr} v(r)\right) e^{v(r)}}{2}, (2, 1, 2) = r, (2, 2, 1) = r, (2, 3, 3) = -r^2 \sin(\theta) \cos(\theta), (3, 1, 3) \\ &= r \sin(\theta)^2, (3, 2, 3) = r^2 \sin(\theta) \cos(\theta), (3, 3, 1) = r \sin(\theta)^2, (3, 3, 2) \\ &= r^2 \sin(\theta) \cos(\theta), (4, 1, 4) = -\frac{\left(\frac{d}{dr} v(r)\right) e^{v(r)}}{2}, (4, 4, 1) = -\frac{\left(\frac{d}{dr} v(r)\right) e^{v(r)}}{2} \left. \right\} \end{aligned} \quad (10)$$

> *Riemann[definition]*

$$R_{\alpha, \beta, \mu, \nu} = g_{\alpha, \lambda} \left( \partial_{\mu} \left( \Gamma_{\beta, \nu}^{\lambda} \right) - \partial_{\nu} \left( \Gamma_{\beta, \mu}^{\lambda} \right) + \Gamma_{\nu, \mu}^{\lambda} \Gamma_{\beta, \nu}^{\nu} - \Gamma_{\nu, \nu}^{\lambda} \Gamma_{\beta, \mu}^{\nu} \right) \quad (11)$$

> *Riemann[nonzero]*

$$\begin{aligned} R_{\alpha, \beta, \mu, \nu} &= \left\{ (1, 2, 1, 2) = \frac{-\left(\frac{d}{dr} b(r)\right) r + b(r)}{-2r + 2b(r)}, (1, 2, 2, 1) = \frac{-\left(\frac{d}{dr} b(r)\right) r + b(r)}{2r - 2b(r)}, (1, \right. \\ 3, 1, 3) &= \frac{\left(-\left(\frac{d}{dr} b(r)\right) r + b(r)\right) \sin(\theta)^2}{-2r + 2b(r)}, (1, 3, 3, 1) = \\ &= \frac{\left(-\left(\frac{d}{dr} b(r)\right) r + b(r)\right) \sin(\theta)^2}{-2r + 2b(r)}, (1, 4, 1, 4) = \frac{1}{4r(r - b(r))} \left( \left( 2r(r \right. \right. \\ &- b(r)) \left( \frac{d^2}{dr^2} v(r) \right) + \left( \frac{d}{dr} v(r) \right) \left( r(r - b(r)) \left( \frac{d}{dr} v(r) \right) - \left( \frac{d}{dr} b(r) \right) r \right. \\ &+ b(r) \left. \right) e^{v(r)} \right), (1, 4, 4, 1) = -\frac{1}{4r(r - b(r))} \left( \left( 2r(r - b(r)) \left( \frac{d^2}{dr^2} v(r) \right) \right. \right. \\ &+ \left( \frac{d}{dr} v(r) \right) \left( r(r - b(r)) \left( \frac{d}{dr} v(r) \right) - \left( \frac{d}{dr} b(r) \right) r + b(r) \right) e^{v(r)} \right), (2, 1, 1, 2) \\ &= \frac{-\left(\frac{d}{dr} b(r)\right) r + b(r)}{2r - 2b(r)}, (2, 1, 2, 1) = \frac{-\left(\frac{d}{dr} b(r)\right) r + b(r)}{-2r + 2b(r)}, (2, 3, 2, 3) \end{aligned} \quad (12)$$

$$\begin{aligned}
&= r \sin(\theta)^2 b(r), (2, 3, 3, 2) = -r \sin(\theta)^2 b(r), (2, 4, 2, 4) = \\
&-\frac{(-r + b(r)) \left( \frac{d}{dr} v(r) \right) e^{v(r)}}{2}, (2, 4, 4, 2) = \frac{(-r + b(r)) \left( \frac{d}{dr} v(r) \right) e^{v(r)}}{2}, (3, 1, \\
&1, 3) = -\frac{\left( -\left( \frac{d}{dr} b(r) \right) r + b(r) \right) \sin(\theta)^2}{-2r + 2b(r)}, (3, 1, 3, 1) \\
&= \frac{\left( -\left( \frac{d}{dr} b(r) \right) r + b(r) \right) \sin(\theta)^2}{-2r + 2b(r)}, (3, 2, 2, 3) = -r \sin(\theta)^2 b(r), (3, 2, 3, 2) \\
&= r \sin(\theta)^2 b(r), (3, 4, 3, 4) = -\frac{\sin(\theta)^2 (-r + b(r)) \left( \frac{d}{dr} v(r) \right) e^{v(r)}}{2}, (3, 4, 4, 3) \\
&= \frac{\sin(\theta)^2 (-r + b(r)) \left( \frac{d}{dr} v(r) \right) e^{v(r)}}{2}, (4, 1, 1, 4) = -\frac{1}{4r(r - b(r))} \left( \left( 2r(r \right. \right. \\
&- b(r)) \left( \frac{d^2}{dr^2} v(r) \right) + \left( \frac{d}{dr} v(r) \right) \left( r(r - b(r)) \left( \frac{d}{dr} v(r) \right) - \left( \frac{d}{dr} b(r) \right) r \right. \\
&+ b(r)) \left. \left. \right) e^{v(r)} \right), (4, 1, 4, 1) = \frac{1}{4r(r - b(r))} \left( \left( 2r(r - b(r)) \left( \frac{d^2}{dr^2} v(r) \right) \right. \right. \\
&+ \left( \frac{d}{dr} v(r) \right) \left( r(r - b(r)) \left( \frac{d}{dr} v(r) \right) - \left( \frac{d}{dr} b(r) \right) r + b(r) \right) \left. \left. \right) e^{v(r)} \right), (4, 2, 2, 4) \\
&= \frac{(-r + b(r)) \left( \frac{d}{dr} v(r) \right) e^{v(r)}}{2}, (4, 2, 4, 2) = -\frac{(-r + b(r)) \left( \frac{d}{dr} v(r) \right) e^{v(r)}}{2}, (4, \\
&3, 3, 4) = \frac{\sin(\theta)^2 (-r + b(r)) \left( \frac{d}{dr} v(r) \right) e^{v(r)}}{2}, (4, 3, 4, 3) = \\
&-\frac{\sin(\theta)^2 (-r + b(r)) \left( \frac{d}{dr} v(r) \right) e^{v(r)}}{2} \left. \right\}
\end{aligned}$$

> Ricci[definition]

$$R_{\mu, \nu} = \partial_{\alpha} \left( \Gamma_{\mu, \nu}^{\alpha} \right) - \partial_{\nu} \left( \Gamma_{\mu, \alpha}^{\alpha} \right) + \Gamma_{\mu, \nu}^{\beta} \Gamma_{\beta, \alpha}^{\alpha} - \Gamma_{\mu, \alpha}^{\beta} \Gamma_{\nu, \beta}^{\alpha}$$

(13)

> Ricci[nonzero]

$$\begin{aligned}
 R_{\mu, \nu} = & \left\{ (1, 1) = \frac{1}{4 r^2 (r - b(r))} \left( -2 r^2 (r - b(r)) \left( \frac{d^2}{dr^2} v(r) \right) - r^2 (r - b(r)) \left( \frac{d}{dr} v(r) \right)^2 + r \left( \left( \frac{d}{dr} b(r) \right) r - b(r) \right) \left( \frac{d}{dr} v(r) \right) + 4 \left( \frac{d}{dr} b(r) \right) r - 4 b(r) \right), (2, 2) \right. \\
 & = \frac{-r (r - b(r)) \left( \frac{d}{dr} v(r) \right) + \left( \frac{d}{dr} b(r) \right) r + b(r)}{2 r}, (3, 3) = \\
 & - \frac{\sin(\theta)^2 \left( r (r - b(r)) \left( \frac{d}{dr} v(r) \right) - \left( \frac{d}{dr} b(r) \right) r - b(r) \right)}{2 r}, (4, 4) \\
 & = \frac{1}{4 r^2} \left( \left( 2 r (r - b(r)) \left( \frac{d^2}{dr^2} v(r) \right) + \left( \frac{d}{dr} v(r) \right) \left( r (r - b(r)) \left( \frac{d}{dr} v(r) \right) - \left( \frac{d}{dr} b(r) \right) r + 4 r - 3 b(r) \right) \right) e^{v(r)} \right) \Big\}
 \end{aligned} \tag{14}$$

> Ricci[scalars]

$$\begin{aligned}
 \Phi_{00} = & \frac{e^{-v(r)} e^{v(r)} \left( r (r - b(r)) \left( \frac{d}{dr} v(r) \right) + \left( \frac{d}{dr} b(r) \right) r - b(r) \right)}{4 r^3}, \Phi_{01} = 0, \Phi_{02} = 0, \\
 \Phi_{11} = & \frac{1}{16 r^3} \left( \left( 2 r^2 (r - b(r)) \left( \frac{d^2}{dr^2} v(r) \right) + r^2 (r - b(r)) \left( \frac{d}{dr} v(r) \right)^2 + \left( \frac{d}{dr} b(r) \right) r^2 + b(r) r \right) \left( \frac{d}{dr} v(r) \right) + 4 b(r) \right) e^{-v(r)} e^{v(r)}, \Phi_{12} = 0, \Phi_{22} \\
 = & \frac{e^{-v(r)} e^{v(r)} \left( r (r - b(r)) \left( \frac{d}{dr} v(r) \right) + \left( \frac{d}{dr} b(r) \right) r - b(r) \right)}{4 r^3}, \Lambda = \frac{1}{48 r^2} \left( \right. \\
 & -2 r (r - b(r)) \left( \frac{d^2}{dr^2} v(r) \right) - r (r - b(r)) \left( \frac{d}{dr} v(r) \right)^2 + \left( \left( \frac{d}{dr} b(r) \right) r - 4 r + 3 b(r) \right) \left( \frac{d}{dr} v(r) \right) + 4 \frac{d}{dr} b(r) \Big)
 \end{aligned} \tag{15}$$

> Einstein[definition]

$$G_{\mu, \nu} = R_{\mu, \nu} - \frac{g_{\mu, \nu} R_{\alpha}^{\alpha}}{2} \tag{16}$$

> Einstein[nonzero]

$$G_{\mu, v} = \left\{ (1, 1) = \frac{r (r - b(r)) \left( \frac{d}{dr} v(r) \right) - b(r)}{r^2 (r - b(r))}, (2, 2) = \frac{1}{4r} \left( 2r^2 (r - b(r)) \left( \frac{d^2}{dr^2} v(r) \right) + \left( r (r - b(r)) \left( \frac{d}{dr} v(r) \right) - \left( \frac{d}{dr} b(r) \right) r + b(r) \right) \left( \left( \frac{d}{dr} v(r) \right) r + 2 \right) \right), (3, 3) = \frac{1}{4r} \left( \sin(\theta)^2 \left( 2r^2 (r - b(r)) \left( \frac{d^2}{dr^2} v(r) \right) + \left( r (r - b(r)) \left( \frac{d}{dr} v(r) \right) - \left( \frac{d}{dr} b(r) \right) r + b(r) \right) \left( \left( \frac{d}{dr} v(r) \right) r + 2 \right) \right) \right), (4, 4) = \frac{e^{v(r)} \left( \frac{d}{dr} b(r) \right)}{r^2} \right\} \quad (17)$$